#################################################################
# Catena-X "Common" Domain Ontology in TTL/RDF/OWL FORMAT
# See copyright notice in the top folder
# See authors file in the top folder
# See license file in the top folder
#################################################################

@prefix : <https://github.com/catenax-ng/product-knowledge/ontology/cx.ttl#> .
@prefix cx: <https://github.com/catenax-ng/product-knowledge/ontology/cx.ttl#> .
@prefix owl: <http://www.w3.org/2002/07/owl#> .
@prefix rdf: <http://www.w3.org/1999/02/22-rdf-syntax-ns#> .
@prefix xml: <http://www.w3.org/XML/1998/namespace> .
@prefix xsd: <http://www.w3.org/2001/XMLSchema#> .
@prefix rdfs: <http://www.w3.org/2000/01/rdf-schema#> .
@base <https://github.com/catenax-ng/product-knowledge/ontology/cx.ttl#> .

cx: rdf:type owl:Ontology ;
    rdfs:comment "The Catena-X Common Domain lists all domain-independent concepts, attributes and relations.â€š"@en ;
    rdfs:label "Catena-X Common Domain" ;
    owl:versionInfo "0.5.1" .

cx:BusinessPartner rdf:type owl:Class ;
    rdfs:comment "A Business Partner is a legal entity that is part of the Catena-X network or that stands in a relevant relation to a Catena-X Business Partner."@en ;
    rdfs:label "Business Partner" .

cx:BPNLType rdf:type rdfs:Datatype ;
    rdfs:comment "The (long) Business Partner Number Type describes strings following the pattern 'BPNL[0-9]{8}[A-Z]{4}'."@en ;
    rdfs:label "Business Partner Number Long Type" ;
    owl:onDatatype xsd:string ;
    owl:withRestrictions ([ xsd:pattern "BPNL[0-9]{8}[A-Z]{4}" ]) .

cx:BPNL rdf:type owl:DatatypeProperty ;
    rdfs:comment "The (long) Business Partner Number is a unique identifier following the pattern 'BPNL[0-9]{8}[A-Z]{4}'."@en ;
    rdfs:label "Business Partner Number Long" ;
    rdfs:domain cx:BusinessPartner ;
    rdfs:range cx:BPNLType .

cx:Asset rdf:type owl:Class ;
    rdfs:comment "An Asset is any artifact that is provisioned/owned/attributed to some Catena-X Business Partner."@en ;
    rdfs:label "Asset" .

cx:provisionedBy rdf:type owl:ObjectProperty;
    rdfs:comment "The provisioned by predicate connects assets to their providing Catena-X Business Partner."@en ;
    rdfs:label "Provisioned By" ;
    rdfs:domain cx:Asset ;
    rdfs:range cx:BusinessPartner .

###  Generated by the OWL API (version 4.5.9.2019-02-01T07:24:44Z) https://github.com/owlcs/owlapi
