#################################################################
# Catena-X "Diagnosis" Domain Ontology in TTL/RDF/OWL FORMAT
# See copyright notice in the top folder
# See authors file in the top folder
# See license file in the top folder
#################################################################

@prefix : <https://github.com/catenax-ng/product-knowledge/ontology/fx.ttl#> .
@prefix cx: <https://github.com/catenax-ng/product-knowledge/ontology/cx.ttl#> .
@prefix cx-fx: <https://github.com/catenax-ng/product-knowledge/ontology/fx.ttl#> .
@prefix owl: <http://www.w3.org/2002/07/owl#> .
@prefix rdf: <http://www.w3.org/1999/02/22-rdf-syntax-ns#> .
@prefix xml: <http://www.w3.org/XML/1998/namespace> .
@prefix xsd: <http://www.w3.org/2001/XMLSchema#> .
@prefix rdfs: <http://www.w3.org/2000/01/rdf-schema#> .
@prefix dcterms: <http://purl.org/dc/terms/> .
@base <https://github.com/catenax-ng/product-knowledge/ontology/fx.ttl#> .

cx-fx: rdf:type owl:Ontology ;
    dcterms:description "The Catena-X Function Domain describes functional declarations."@en ;
    dcterms:title "Catena-X Function Domain" ;
    owl:versionInfo "0.5.2" .

cx-fx:Function rdf:type owl:Class ;
    dcterms:description "A Function is a (reified) relation mapping a domain of arguments (inputs) to a unique tuple of return values (outputs). Instances are the individual invocations."@en ;
    dcterms:title "Function".

cx-fx:Argument rdf:type owl:Class ;
    dcterms:description "A (Function) Argument describes a mapping from an instance (literal) to the invocation."@en ;
    dcterms:title "Argument".

cx-fx:ReturnValue rdf:type owl:Class ;
    dcterms:description "A (Functional) Return Value describes a mapping an invocation result to an instance (variable)."@en ;
    dcterms:title "Return Value".

cx-fx:targetUri rdf:type owl:DatatypeProperty ;
    dcterms:description "The Target URI of a function describes the actual endpoint which realizes the function. Only needed in implementation descriptions."@en ;
    dcterms:title "Target Uri" ;
    rdfs:domain cx-fx:Function ;
    rdfs:range xsd:string .

cx-fx:invocationMethod rdf:type owl:DatatypeProperty ;
    dcterms:description "The Invocation Method of a function describes how the actual endpoint is called. Only needed in implementation descriptions."@en ;
    dcterms:title "Invocation Method" ;
    rdfs:domain cx-fx:Function ;
    rdfs:range xsd:string .

cx-fx:argumentName rdf:type owl:DatatypeProperty ;
    dcterms:description "The Argument Name of an argument maps a node to an actual endpoint argument. Only needed in implementation descriptions."@en ;
    dcterms:title "Argument Name" ;
    rdfs:domain cx-fx:Argument ;
    rdfs:range xsd:string .

cx-fx:valuePath rdf:type owl:DatatypeProperty ;
    dcterms:description "The Value Path of a return value maps a well-defined part of the endpoint response to a node in the graph. Only needed in implementation descriptions."@en ;
    dcterms:title "Value Path" ;
    rdfs:domain cx-fx:ReturnValue ;
    rdfs:range xsd:string .

cx-fx:dataType rdf:type owl:ObjectProperty ;
    dcterms:description "The Data Type of a return value maps a well-defined part of the endpoint response to a node in the graph. Only needed in implementation descriptions."@en ;
    dcterms:title "Value Path" ;
    rdfs:domain cx-fx:ReturnValue ;
    rdfs:range rdfs:Datatype.

cx-fx:input rdf:type owl:ObjectProperty ;
    dcterms:description "The Input property relates invocations to their arguments."@en ;
    dcterms:title "Input" ;
    rdfs:domain cx-fx:Function ;
    rdfs:range rdfs:Argument.

cx-fx:output rdf:type owl:ObjectProperty ;
    dcterms:description "The Output property relates invocations to their return values."@en ;
    dcterms:title "Output" ;
    rdfs:domain cx-fx:Function ;
    rdfs:range rdfs:ReturnValue.

###  Generated by the OWL API (version 4.5.9.2019-02-01T07:24:44Z) https://github.com/owlcs/owlapi
